src/ka.v
@@ -1,9 +1,18 @@
 (** * gnl_alg.ka : Classic encoding of Kleene algebra *)
 Require Import prelim.
-
-
+(** We provide here a standard representation of Kleene algebra, as the algebra *)
+(** of regular expressions interpreted as languages, i.e. predicates over lists. *)
+  
 Section reg.
+
+  (** * Syntax & axiomatisation *)
+
+  (** We fix a decidable set [A]. *)
+  
   Context {A : Set}{decA:decidable_set A}.
+
+  (** Regular expressions are built out of variables from [A], the constants [0r] and [1r], *)
+  (** as well as two binary operators [+r] and [×r] and a unary operator [^*]. *)
   
   Inductive reg :=
   | r_var : A -> reg
@@ -18,47 +27,48 @@ Section reg.
   Infix "+r" := r_sum (at level 20).
   Infix "×r" := r_prod (at level 20).
   Notation " e ^* " := (r_star e).
-  
 
-  Fixpoint support (e : reg) : list A :=
-    match e with
-    | 1r | 0r => []
-    | r_var a => [a]
-    | e^* => support e
-    | e1 ×r e2 | e1 +r e2 => support e1 ++ support e2
-    end.
+  (** We define the axiomatic equivalence [=KA] as follows: *)
   
-  Definition Sum : list reg -> reg :=
-    fold_right r_sum 0r.
-
   Reserved Notation " e =KA f" (at level 60).
   
   Inductive KA_eq : relation reg :=
+  (** It is an equivalence relation, i.e. reflexive symmetric and transitive. *)
   | KA_eq_refl e : e =KA e
   | KA_eq_sym e f : e =KA f -> f =KA e
   | KA_eq_trans e f g : e =KA f -> f =KA g -> e =KA g
+  (** It is a congruence with respect to each operator. *)
   | KA_eq_prod e1 f1 e2 f2 : e1 =KA e2 -> f1 =KA f2 -> e1 ×r f1 =KA e2 ×r f2
   | KA_eq_sum e1 f1 e2 f2 : e1 =KA e2 -> f1 =KA f2 -> e1 +r f1 =KA e2 +r f2
   | KA_eq_star e1 e2 : e1 =KA e2 -> e1^* =KA e2^*
+  (** Both binary operators are associative. *)
   | KA_eq_prod_assoc e f g : e ×r (f ×r g) =KA (e ×r f) ×r g
   | KA_eq_sum_assoc e f g : e +r (f +r g) =KA (e +r f) +r g
+  (** [+r] is commutative and idempotent. *)
   | KA_eq_sum_comm e f : e +r f =KA f +r e
   | KA_eq_sum_idem e : e +r e =KA e
+  (** [1r] is the unit of [×r] and [0r] that of [+r]. *)
   | KA_eq_prod_one_e e : 1r ×r e =KA e
   | KA_eq_prod_e_one e : e ×r 1r =KA e
   | KA_eq_sum_zero_e e : 0r +r e =KA e
+  (** [×r] distributes over [+r]. *)
   | KA_eq_prod_sum e f g : e ×r (f +r g) =KA (e ×r f) +r (e ×r g)
   | KA_eq_sum_prod e f g : (e +r f) ×r g =KA (e ×r g) +r (f ×r g)
+  (** [0r] is an annihilator for [×r]. *)
   | KA_eq_prod_zero e : e ×r 0r =KA 0r
   | KA_eq_zero_prod e : 0r ×r e =KA 0r
+  (** [^*] may be unfolded on both sides. *)
   | KA_eq_star_unfold_left e : e^* =KA 1r +r (e ×r (e^* ))
   | KA_eq_star_unfold_right e : e^* =KA 1r +r ((e^* ) ×r e)
+  (** [^*] enjoys two _induction axioms_ :*)
   | KA_eq_star_left_ind e f : (e ×r f) +r f =KA f -> ((e^* ) ×r f) +r f =KA f
   | KA_eq_star_right_ind e f : (f ×r e) +r f =KA f -> (f ×r (e^* )) +r f =KA f
   where " e =KA f " := (KA_eq e f).
-                                                                  
+               
   Hint Constructors KA_eq : proofs.
 
+  (** Some obvious properties of this relation. *)
+  
   Global Instance KA_eq_equiv : Equivalence KA_eq.
   Proof.
     split.
@@ -80,6 +90,7 @@ Section reg.
   Global Instance r_star_proper : Proper (KA_eq ==> KA_eq) r_star.
   Proof. intros s s' es;apply KA_eq_star;assumption. Qed.
 
+  (** An associated preorder is defined by [e≤f] iff [e+f=f]. *)
    
   Definition KA_inf : relation reg := fun e f => e +r f =KA f.
 
@@ -95,6 +106,9 @@ Section reg.
       + rewrite KA_eq_sum_assoc.
         rewrite h1,h2;reflexivity.
   Qed.
+
+  (** [≤KA] is a partial order w.r.t. [=KA]. *)
+  
   Global Instance KA_inf_partialorder : PartialOrder KA_eq KA_inf.
   Proof.
     intros e f;unfold Basics.flip,KA_inf;split.
@@ -103,6 +117,26 @@ Section reg.
       rewrite <- E1,KA_eq_sum_comm,E2.
       reflexivity.
   Qed.
+
+  (** [+r] is a join operator for the preorder [≤KA]. *)
+  
+  Lemma KA_inf_join_l e f : e ≤KA e +r f.
+  Proof. unfold KA_inf;rewrite KA_eq_sum_assoc,KA_eq_sum_idem;reflexivity. Qed.
+
+  Lemma KA_inf_join_r e f : f ≤KA e +r f.
+  Proof. unfold KA_inf;rewrite KA_eq_sum_comm,<-KA_eq_sum_assoc,KA_eq_sum_idem;reflexivity. Qed.
+
+  Lemma KA_inf_join e f g : e ≤KA g -> f ≤KA g -> e +r f ≤KA g.
+  Proof. unfold KA_inf;intros h1 h2;rewrite <- h1,<- h2 at 2;symmetry;apply KA_eq_sum_assoc. Qed.
+
+  Lemma KA_inf_sum_l e f g : e ≤KA f -> e ≤KA f +r g.
+  Proof. intros ->;apply KA_inf_join_l. Qed.
+
+  Lemma KA_inf_sum_r e f g : e ≤KA g -> e ≤KA f +r g.
+  Proof. intros ->;apply KA_inf_join_r. Qed.
+
+  (** Every operator is monotonous w.r.t. [≤KA]. *)
+
   Global Instance r_prod_mono : Proper (KA_inf ==> KA_inf ==> KA_inf) r_prod.
   Proof.
     unfold KA_inf;intros e1 e2 he f1 f2 hf.
@@ -128,33 +162,48 @@ Section reg.
     repeat rewrite KA_eq_sum_assoc.
     reflexivity.
   Qed.
-  Lemma KA_inf_join_l e f : e ≤KA e +r f.
-  Proof. unfold KA_inf;rewrite KA_eq_sum_assoc,KA_eq_sum_idem;reflexivity. Qed.
-  Lemma KA_inf_join_r e f : f ≤KA e +r f.
-  Proof. unfold KA_inf;rewrite KA_eq_sum_comm,<-KA_eq_sum_assoc,KA_eq_sum_idem;reflexivity. Qed.
-  Lemma KA_inf_join e f g : e ≤KA g -> f ≤KA g -> e +r f ≤KA g.
-  Proof. unfold KA_inf;intros h1 h2;rewrite <- h1,<- h2 at 2;symmetry;apply KA_eq_sum_assoc. Qed.
 
-  Lemma KA_inf_sum_l e f g : e ≤KA f -> e ≤KA f +r g.
-  Proof. intros ->;apply KA_inf_join_l. Qed.
-  Lemma KA_inf_sum_r e f g : e ≤KA g -> e ≤KA f +r g.
-  Proof. intros ->;apply KA_inf_join_r. Qed.
+  Global Instance r_star_mono : Proper (KA_inf ==> KA_inf) r_star.
+  Proof.
+    intros e f h.
+    rewrite KA_eq_star_unfold_left at 1.
+    apply KA_inf_join.
+    - rewrite KA_eq_star_unfold_left;apply KA_inf_join_l.
+    - rewrite h at 1.
+      transitivity (f^*×r e^* );[apply r_prod_mono;[|reflexivity]|].
+      + rewrite KA_eq_star_unfold_left,KA_eq_star_unfold_left.
+        apply KA_inf_sum_r.
+        rewrite <- (KA_eq_prod_e_one) at 1.
+        apply r_prod_mono;[reflexivity|].
+        apply KA_inf_join_l.
+      + apply KA_eq_star_right_ind.
+        cut (f ^* ×r e ≤KA f ^* );[intro h';apply h'|].
+        rewrite h.
+        rewrite KA_eq_star_unfold_right at 2.
+        apply KA_inf_join_r.
+  Qed.
+
+  (** Below is a collection of useful facts about [=KA] and [≤KA]. *)
 
   Lemma KA_inf_zero e : 0r ≤KA e.
   Proof. unfold KA_inf;auto with proofs. Qed.
   
   Lemma KA_inf_star_one e : 1r ≤KA e^* .
   Proof. rewrite KA_eq_star_unfold_left;apply KA_inf_join_l. Qed.
+
   Lemma KA_inf_star_e e : e ≤KA e^* .
   Proof.
     rewrite KA_eq_star_unfold_left.
     rewrite <- KA_inf_star_one,KA_eq_prod_e_one.
     apply KA_inf_join_r.
   Qed.
+
   Lemma KA_inf_star_left_ind e f : e ×r f ≤KA f -> (e^* ) ×r f ≤KA f.
   Proof. apply (KA_eq_star_left_ind e f). Qed.
+
   Lemma KA_inf_star_right_ind e f : f ×r e ≤KA f -> f ×r (e^* ) ≤KA f.
   Proof. apply (KA_eq_star_right_ind e f). Qed.
+
   Lemma KA_inf_star_ind e f : e ×r (f^* ) ≤KA f^* -> e^* ≤KA f^*.
   Proof.
     intro h;apply KA_inf_star_left_ind in h as <-.
@@ -180,15 +229,6 @@ Section reg.
       reflexivity.
     - apply KA_inf_star_e.
   Qed.
-  
-  Global Instance r_star_mono : Proper (KA_inf ==> KA_inf) r_star.
-  Proof.
-    intros e f h.
-    apply KA_inf_star_ind.
-    rewrite h.
-    rewrite KA_eq_star_unfold_left at 2.
-    apply KA_inf_join_r.
-  Qed.
 
   Lemma KA_eq_star_sum_one (e : reg) : (1r +r e)^* =KA e^*.
   Proof.
@@ -201,19 +241,34 @@ Section reg.
     - rewrite <- KA_inf_join_r;reflexivity.
   Qed.
 
+  (** * Semantics *)
+
+  (** We now define the language associated with an expression, through a satisfaction *)
+  (** predicate [l |=KA e], specifying when a list [l] belongs to the language associated *)
+  (** with an expression [e]. *)
+  
   Reserved Notation " l |=KA e " (at level 60).
   
   Fixpoint KA_sat (l : list A) (e : reg) : Prop :=
     match e with
+    (** The language of [0r] is empty. *)
     | 0r => False
+    (** Only the empty list satisfies [1r]. *)
     | 1r => l = []
+    (** Variables are satisfied by singleton lists. *)
     | r_var a => l = [a]
+    (** Lists satisfying [e ×r f] are concatenations of a list satisfying [e] and one *)
+    (** satisfying [f]. *)
     | e ×r f => exists l1 l2, l = l1 ++ l2 /\ l1 |=KA e /\ l2 |=KA f
+    (** The language of [e +r f] is the union of the languages of [e] and [f]. *)
     | e +r f => l |=KA e \/ l |=KA f
+    (** A list satisfies [e^*] if it can be written as a concatenation of lists that *)
+    (** all satisfy [e]. *)
     | e^* => exists L, l = concat L /\ forall k, In k L -> k |=KA e
     end
   where " l |=KA e " := (KA_sat l e).
-  
+
+  (** The axioms of the previous section are sound w.r.t. this semantic interpretation. *)
   Global Instance KA_sound s : Proper (KA_eq ==> iff) (KA_sat s).
   Proof.
     intros e f pr;revert s;induction pr;intro s;simpl;try now firstorder.
@@ -315,123 +370,86 @@ Section reg.
   Global Instance KA_inf_sound s : Proper (KA_inf ==> Basics.impl) (KA_sat s).
   Proof. intros e f he h;unfold KA_inf in he;rewrite <- he;now left. Qed.
 
-  Lemma Sum_sat w L : w |=KA Sum L <-> exists e, w |=KA e /\ In e L.
-  Proof.
-    induction L;simpl;firstorder.
-    subst;tauto.
-  Qed.
+  (** * Empty word property *)
 
-  Lemma Sum_join_In e L : In e L -> e ≤KA Sum L.
-  Proof.
-    induction L;simpl;[tauto|].
-    intros [<-|h];[apply KA_inf_sum_l|apply KA_inf_sum_r];auto.
-    reflexivity.
-  Qed.
-
-  Lemma Sum_join_inf e L : Forall (fun f => f ≤KA e) L -> Sum L ≤KA e.
-  Proof.
-    revert e;induction L as [|f L];intros e hyp.
-    - unfold KA_inf;auto with proofs.
-    - apply Forall_cons_iff in hyp as (hypf&hypL).
-      simpl;apply KA_inf_join;auto.
-  Qed.
+  (** It will be useful to be able to identify which expressions satisfy the so-called *)
+  (** _empty word property_ (ewp), i.e. expressions [e] such that [[] |=KA e]. We do so *)
+  (** using the following boolean predicate. *)
   
-  Section ewp.
-    Fixpoint r_ewp (e : reg) : bool :=
-      match e with
-      | r_var _ | 0r => false
-      | _ ^* | 1r => true
-      | e ×r f => r_ewp e && r_ewp f
-      | e +r f => r_ewp e || r_ewp f
-      end.
+  Fixpoint r_ewp (e : reg) : bool :=
+    match e with
+    | r_var _ | 0r => false
+    | _ ^* | 1r => true
+    | e ×r f => r_ewp e && r_ewp f
+    | e +r f => r_ewp e || r_ewp f
+    end.
 
-    Lemma r_ewp_spec e : r_ewp e = true -> [] |=KA e.
-    Proof.
-      induction e;simpl;try reflexivity||discriminate.
-      - rewrite Bool.andb_true_iff.
-        intros (h1&h2);exists [],[];repeat split;auto.
-      - rewrite Bool.orb_true_iff.
-        intros [h|h];auto.
-      - intros _;exists [];split;auto.
-        intros k f;exfalso;apply f.
-    Qed.
+  (** To establish the correctness of [r_ewp], we first show that it is a morphism from *)
+  (** expressions up-to [=KA] to the booleans (up-to equality). *)
+ 
+  Lemma r_ewp_eq : Proper (KA_eq ==> eq) r_ewp.
+  Proof.
+    intros e f pr;induction pr;simpl;try reflexivity||(now f_equal)||eauto.
+    - apply Bool.andb_assoc.
+    - apply Bool.orb_assoc.
+    - apply Bool.orb_comm.
+    - apply Bool.orb_diag.
+    - apply Bool.andb_true_r.
+    - apply Bool.andb_orb_distrib_r.
+    - apply Bool.andb_orb_distrib_l.
+    - apply Bool.andb_false_r.
+    - apply Bool.orb_diag.
+    - rewrite Bool.andb_true_r.
+      apply Bool.orb_diag.
+  Qed.
 
-    Lemma r_ewp_eq : Proper (KA_eq ==> eq) r_ewp.
-    Proof.
-      intros e f pr;induction pr;simpl;try reflexivity||(now f_equal)||eauto.
-      - apply Bool.andb_assoc.
-      - apply Bool.orb_assoc.
-      - apply Bool.orb_comm.
-      - apply Bool.orb_diag.
-      - apply Bool.andb_true_r.
-      - apply Bool.andb_orb_distrib_r.
-      - apply Bool.andb_orb_distrib_l.
-      - apply Bool.andb_false_r.
-      - apply Bool.orb_diag.
-      - rewrite Bool.andb_true_r.
-        apply Bool.orb_diag.
-    Qed.
+  (** We can now establish that [r_ewp e] is [true] exactly when the empty list *)
+  (** satisfies the expression [e]. *)
+  
+  Lemma r_ewp_spec e :
+    r_ewp e = true <-> [] |=KA e.
+  Proof.
+    split;induction e;simpl;try reflexivity||discriminate||tauto.
+    - rewrite Bool.andb_true_iff.
+      intros (h1&h2);exists [],[];repeat split;auto.
+    - rewrite Bool.orb_true_iff.
+      intros [h|h];auto.
+    - intros _;exists [];split;auto.
+      intros k f;exfalso;apply f.
+    - intros (l1&l2&E&h1&h2).
+      symmetry in E.
+      apply app_eq_nil in E as (->&->).
+      rewrite IHe1,IHe2 by assumption.
+      reflexivity.
+    - rewrite Bool.orb_true_iff.
+      tauto.
+  Qed.
 
-    Lemma r_ewp_spec_iff e :
-      r_ewp e = true <-> [] |=KA e.
-    Proof.
-      split;[apply r_ewp_spec|].
-      induction e;simpl;try discriminate||tauto.
-      - intros (l1&l2&E&h1&h2).
-        symmetry in E.
-        apply app_eq_nil in E as (->&->).
-        rewrite IHe1,IHe2 by assumption.
+  (** Alternatively, we can specfiy [r_ewp] by stating that this predicate characterizes *)
+  (** expressions that are above [1r] in the preorder [≤KA]. *)
+  
+  Lemma r_ewp_alt_spec e :
+    r_ewp e = true <-> 1r ≤KA e.
+  Proof.
+    split.
+    - induction e;simpl;try reflexivity||discriminate.
+      + rewrite Bool.andb_true_iff.
+        intros (h1&h2);apply IHe1 in h1;apply IHe2 in h2.
+        rewrite <- h1,<- h2.
+        repeat rewrite KA_eq_sum_prod||rewrite KA_eq_prod_sum
+               ||rewrite KA_eq_prod_e_one||rewrite KA_eq_prod_one_e.
         reflexivity.
-      - rewrite Bool.orb_true_iff.
-        tauto.
-    Qed.
-
-    Lemma r_ewp_eq_iff e :
-      r_ewp e = true <-> e +r 1r =KA e.
-    Proof.
-      split.
-      - induction e;simpl;try reflexivity||discriminate.
-        + intros _;apply KA_eq_sum_idem.
-        + rewrite Bool.andb_true_iff.
-          intros (h1&h2);apply IHe1 in h1;apply IHe2 in h2.
-          rewrite <- h1,<- h2.
-          repeat rewrite KA_eq_sum_prod||rewrite KA_eq_prod_sum
-                 ||rewrite KA_eq_prod_e_one||rewrite KA_eq_prod_one_e.
-          repeat rewrite <- KA_eq_sum_assoc.
-          rewrite KA_eq_sum_idem.
-          reflexivity.
-        + rewrite Bool.orb_true_iff.
-          intros [h|h];auto.
-          * apply IHe1 in h.
-            rewrite <- h.
-            repeat rewrite KA_eq_sum_prod||rewrite KA_eq_prod_sum
-                   ||rewrite KA_eq_prod_e_one||rewrite KA_eq_prod_one_e.
-            repeat rewrite <- KA_eq_sum_assoc.
-            repeat rewrite (KA_eq_sum_comm 1r).
-            repeat rewrite <- KA_eq_sum_assoc.
-            rewrite KA_eq_sum_idem.
-            reflexivity.
-          * apply IHe2 in h.
-            rewrite <- h.
-            repeat rewrite KA_eq_sum_prod||rewrite KA_eq_prod_sum
-                   ||rewrite KA_eq_prod_e_one||rewrite KA_eq_prod_one_e.
-            repeat rewrite <- KA_eq_sum_assoc.
-            rewrite KA_eq_sum_idem.
-            reflexivity.
-        + intros _.
-          rewrite KA_eq_star_unfold_left.
-          repeat rewrite <- KA_eq_sum_assoc.
-          repeat rewrite (KA_eq_sum_comm 1r).
-          repeat rewrite <- KA_eq_sum_assoc.
-          rewrite KA_eq_sum_idem.
-          reflexivity.
-      - intro E;apply r_ewp_eq in E.
-        simpl in E.
-        rewrite Bool.orb_true_r in E.
-        rewrite <- E;reflexivity.
-    Qed.
-  End ewp.
-
+      + rewrite Bool.orb_true_iff.
+        intros [h|h];auto.
+        * apply IHe1 in h.
+          rewrite <- h.
+          apply KA_inf_join_l.
+        * apply IHe2 in h.
+          rewrite <- h.
+          apply KA_inf_join_r.
+      + intros _;apply KA_inf_star_one.
+    - intro E;apply r_ewp_eq in E as <-;reflexivity.
+  Qed.
  
 End reg.
 
@@ -449,160 +467,3 @@ Hint Constructors KA_eq : proofs.
 Hint Resolve KA_eq_sum_e_zero : proofs.
 
 Arguments reg : clear implicits.
-  
-Section reg_functor.
-  
-  Fixpoint reg_lift {A B : Set} (r : A -> B -> Prop) (e : reg A) (f : reg B) : Prop :=
-    match e,f with
-    | r_var a,r_var b => r a b
-    | 1r,1r | 0r,0r => True
-    | e1 ×r e2,f1 ×r f2 | e1 +r e2,f1 +r f2 => reg_lift r e1 f1 /\ reg_lift r e2 f2
-    | e^*,f^* => reg_lift r e f
-    | _,_ => False
-    end.
-
-  Global Instance reg_lift_equiv {A : Set} {r : relation A} {er : Equivalence r} :
-    Equivalence (reg_lift r).
-  Proof.
-    split.
-    - intros e;induction e;simpl;auto.
-      reflexivity.
-    - intros e;induction e;intros [];simpl;auto.
-      + intro;symmetry;assumption.
-      + intros (h1&h2);split;apply IHe1||apply IHe2;auto.
-      + intros (h1&h2);split;apply IHe1||apply IHe2;auto.
-    - intros e;induction e;intros [] [];simpl;try tauto.
-      + intros;etransitivity;eassumption.
-      + intros (h1&h2) (h3&h4);split;[eapply IHe1|eapply IHe2];eauto.
-      + intros (h1&h2) (h3&h4);split;[eapply IHe1|eapply IHe2];eauto.
-      + intros h1 h2;eapply IHe;eauto.
-  Qed.
-
-  Fixpoint reg_map {A B : Set} (f : A -> B) (e : reg A) : reg B :=
-    match e with 
-    | r_var a => r_var (f a)
-    | 1r => 1r
-    | 0r => 0r
-    | e1 ×r e2 => (reg_map f e1) ×r (reg_map f e2)
-    | e1 +r e2 => (reg_map f e1) +r (reg_map f e2)
-    | e^* => (reg_map f e)^*
-    end.
-
-  Global Instance reg_map_reg_lift {A B : Set} (f : A -> B) (r : relation A) (s : relation B) :
-    Proper (r ==> s) f -> Proper (reg_lift r ==> reg_lift s) (reg_map f).
-  Proof. intros proper e;induction e;intros [];simpl;intuition. Qed.
-
-  
-  Lemma KA_sat_reg_map {X Y : Set} (f : X -> Y) m e :
-    m |=KA reg_map f e <-> exists m', map f m' = m /\ m' |=KA e.
-  Proof.
-    revert m;induction e;simpl;try setoid_rewrite IHe1;try setoid_rewrite IHe2;
-      try (setoid_rewrite IHe;clear IHe);(firstorder subst);try reflexivity.
-    - exists [a];simpl;auto.
-    - exists [];simpl;auto.
-    - exists (x2++x1);rewrite map_app;firstorder.
-    - exists (map f x0),(map f x1);rewrite map_app;firstorder.
-    - induction x.
-      + exists [];split;auto.
-        exists [];simpl;tauto.
-      + simpl.
-        destruct IHx as (m2&<-&L&->&hL);[intros;apply H0;now right|].
-        destruct (H0 a) as (m1&<-&h1);[now left|].
-        exists (m1++concat L);rewrite map_app;firstorder.
-        exists (m1::L);simpl;(firstorder subst);auto.
-    - induction x0.
-      + exists [];simpl;split;tauto.
-      + simpl.
-        rewrite map_app.
-        destruct IHx0 as (L&->&hL);[intros;apply H1;now right|].
-        exists ((map f a)::L);simpl;(firstorder subst);auto.
-  Qed.
-
-  Lemma r_ewp_reg_map {X Y : Set} (f : X -> Y) e : r_ewp (reg_map f e) = r_ewp e.
-  Proof. induction e;simpl;try rewrite IHe1,IHe2||rewrite IHe;auto. Qed.
-
-  Fixpoint Distr {A : Set} (e : reg (list A)) : reg A :=
-    match e with
-    | r_var l => Sum (map r_var l)
-    | 1r => 1r
-    | 0r => 0r
-    | e ×r f => Distr e ×r Distr f
-    | e +r f => Distr e +r Distr f
-    | e^* => (Distr e)^*
-    end.
-
-  Lemma Distr_spec {A : Set} (e : reg (list A)) :
-    forall w, w |=KA (Distr e) <-> exists l, list_lift (@In A) w l /\ l |=KA e.
-  Proof.
-    induction e;simpl.
-    - intro w.
-      rewrite Sum_sat.
-      setoid_rewrite in_map_iff.
-      split;[intros (e&h1&x&<-&h2)|intros (l&h&->)].
-      + exists [a];split;auto.
-        simpl in h1;subst.
-        split;simpl;auto.
-      + destruct w as [|x[]];simpl in h;try tauto.
-        destruct h as (h&_).
-        exists (r_var x);split;simpl;auto.
-        exists x;split;auto.
-    - intros w;split;[intros ->;exists [];split;simpl;auto|intros (l&h&->)].
-      destruct w as [|];simpl in h;try tauto.
-    - now firstorder.
-    - setoid_rewrite IHe1;setoid_rewrite IHe2;clear IHe1 IHe2.
-      intro w;split.
-      + intros (l1&l2&->&(m1&hl1&hm1)&m2&hl2&hm2).
-        exists (m1++m2);split.
-        * apply app_list_lift;assumption.
-        * exists m1,m2;repeat split;auto.
-      + intros (l&hl&l1&l2&->&hl1&hl2).
-        apply list_lift_app in hl as (m1&m2&->&hm1&hm2).
-        firstorder.
-    - now firstorder.
-    - setoid_rewrite IHe;clear IHe.
-      intros w;split.
-      + intros (L&->&hL).
-        induction L;simpl;auto.
-        * exists [];split;auto.
-          exists [];simpl;tauto.
-        * destruct IHL as (l&hl&L'&->&hL').
-          -- intros k hk;apply hL;now right.
-          -- assert (In a (a::L)) as ha by now left.
-             apply hL in ha as (l'&ha&hl').
-             exists (l'++concat L').
-             split;[apply app_list_lift;auto|].
-             exists (l'::L');split;auto.
-             intros k [<-|hk];[|apply hL'];auto.
-      + intros (l&hl&L&->&hL).
-        revert w hl hL;induction L;intros w hw hL;simpl in *.
-        * exists [];split;simpl;[|tauto].
-          destruct w;simpl in hw;tauto.
-        * apply list_lift_app in hw as (l1&l2&->&hl1&hl2).
-          apply IHL in hl2 as (L'&->&hL');[|intros;apply hL;now right].
-          exists (l1::L');split;auto.
-          intros k [<-|hk];[exists a;split|apply hL'];auto.
-  Qed.
-
-  Context  {A : Set} {rA : relation A} {sumA : list A -> A} .
-  Inductive mixed_eq: relation (reg A) :=
-  | meq_refl e : mixed_eq e e
-  | meq_sym e f : mixed_eq e f -> mixed_eq f e
-  | meq_trans e f g : mixed_eq e f -> mixed_eq f g -> mixed_eq e g
-  | meq_ka e f : e =KA f -> mixed_eq e f
-  | meq_r e f : reg_lift rA e f -> mixed_eq e f
-  | meq_Distr E : mixed_eq (Distr E) (reg_map sumA E).
-
-  Hint Constructors mixed_eq : proofs.
-  Global Instance mixed_eq_equiv : Equivalence mixed_eq.
-  Proof. split;intro;intros;eauto with proofs. Qed.
-  
-  Lemma mixed_eq_vars (a b : A) : mixed_eq ((r_var a) +r (r_var b)) (r_var (sumA [a;b])).
-  Proof.
-    transitivity (Distr (r_var [a;b]));[simpl;auto with proofs|].
-    apply meq_Distr.
-  Qed.
-
-  
-End reg_functor.
-Hint Constructors mixed_eq : proofs.
-
